parameric on P Q

flat.v
@@ -1,4 +1,4 @@
-From iris.program_logic Require Export auth weakestpre.
+From iris.program_logic Require Export auth weakestpre saved_prop.
 From iris.proofmode Require Import invariants ghost_ownership.
 From iris.heap_lang Require Export lang.
 From iris.heap_lang Require Import proofmode notation.
@@ -45,84 +45,88 @@ Definition install : val :=
      "p".
 
 Definition mk_flat : val :=
-  λ: <>,
+  λ: "f",
    let: "lk" := newlock #() in
    let: "s" := new_stack #() in
-   λ: "f",
-      λ: "x",
-         let: "p" := install "x" "s" in
-         loop "f" "p" "s" "lk".
+   λ: "x",
+      let: "p" := install "x" "s" in
+      loop "f" "p" "s" "lk".
 
 Global Opaque doOp try_srv install loop mk_flat.
 
 Definition reqR := prodR fracR (dec_agreeR val). (* request x should be kept same *)
-Definition toks : Type := gname * gname * gname * gname. (* a bunch of tokens to do state transition *)
+Definition toks : Type := gname * gname * gname * gname * gname. (* a bunch of tokens to do state transition *)
 Definition tokmR := evmapR loc toks. (* tie each slot to tokens *)
 Definition reqmR := evmapR loc val. (* tie each slot to request value *)
 Class flatG Σ := FlatG {
   req_G :> inG Σ reqR;
   tok_G :> inG Σ (authR tokmR);
+  sp_G  :> savedPropG Σ (cofe_funCF val idCF)
 }.
 
 Definition flatΣ : gFunctors :=
   #[ GFunctor (constRF reqR);
-     GFunctor (constRF (authR tokmR))
+     GFunctor (constRF (authR tokmR));
+     savedPropΣ (cofe_funCF val idCF)
    ].
 
 Instance subG_flatΣ {Σ} : subG flatΣ Σ → flatG Σ.
-Proof. intros [?%subG_inG [?%subG_inG _]%subG_inv]%subG_inv. split; apply _. Qed.
+Proof. intros [?%subG_inG [?%subG_inG [? _]%subG_inv]%subG_inv]%subG_inv. split; apply _. Qed.
 
 Section proof.
   Context `{!heapG Σ, !lockG Σ, !evidenceG loc val Σ, !flatG Σ} (N : namespace).
-  Context (R: iProp Σ) (* private resource *)
-          (P: val → iProp Σ) (* common pre-cond *)
-          (Q: val → val → iProp Σ) (* common post-cond *)
-          `{∀ x, TimelessP (P x), ∀ x y, TimelessP (Q x y)}.
+  Context (R: iProp Σ).
 
-  Definition init_s (ts: toks) := let '(_, γ1, γ3, _) := ts in (own γ1 (Excl ()) ★ own γ3 (Excl ()))%I.
-  Definition installed_s (ts: toks) (x: val) :=
-    let '(γx, γ1, _, γ4) := ts in (own γx ((1/2)%Qp, DecAgree x) ★ P x ★ own γ1 (Excl ()) ★ own γ4 (Excl ()))%I.
+  Definition init_s (ts: toks) :=
+    let '(_, γ1, γ3, _, _) := ts in (own γ1 (Excl ()) ★ own γ3 (Excl ()))%I.
+
+  Definition installed_s (ts: toks) (f x: val) :=
+    let '(γx, γ1, _, γ4, γq) := ts in
+    (∃ (P: val → iProp Σ) Q, own γx ((1/2)%Qp, DecAgree x) ★ P x ★ ({{ R ★ P x }} f x {{ v, R ★ Q x v }}) ★
+                             saved_prop_own γq (Q x) ★ own γ1 (Excl ()) ★ own γ4 (Excl ()))%I.
+
   Definition received_s (ts: toks) (x: val) γr :=
-    let '(γx, _, _, γ4) := ts in (own γx ((1/2/2)%Qp, DecAgree x) ★ own γr (Excl ()) ★ own γ4 (Excl ()))%I.
+    let '(γx, _, _, γ4, _) := ts in
+    (own γx ((1/2/2)%Qp, DecAgree x) ★ own γr (Excl ()) ★ own γ4 (Excl ()))%I.
+
   Definition finished_s (ts: toks) (x y: val) :=
-    let '(γx, γ1, _, γ4) := ts in
-    (own γx ((1/2)%Qp, DecAgree x) ★ Q x y ★ own γ1 (Excl ()) ★ own γ4 (Excl ()))%I.
+    let '(γx, γ1, _, γ4, γq) := ts in
+    (∃ Q: val → val → iProp Σ,
+       own γx ((1/2)%Qp, DecAgree x) ★ saved_prop_own γq (Q x) ★
+       Q x y ★ own γ1 (Excl ()) ★ own γ4 (Excl ()))%I.
 
   Definition evm := ev loc toks.
   
   (* p slot invariant *)
-  Definition p_inv (γm γr: gname) (v: val) :=
+  Definition p_inv (γm γr: gname) (f v: val) :=
     (∃ (ts: toks) (p : loc),
        v = #p ★ evm γm p ts ★
        ((* INIT *)
         (∃ y: val, p ↦{1/2} InjRV y ★ init_s ts)∨
         (* INSTALLED *)
-        (∃ x: val, p ↦{1/2} InjLV x ★ installed_s ts x) ∨
+        (∃ x: val, p ↦{1/2} InjLV x ★ installed_s ts f x) ∨
         (* RECEIVED *)
         (∃ x: val, p ↦{1/2} InjLV x ★ received_s ts x γr) ∨
         (* FINISHED *)
         (∃ x y: val, p ↦{1/2} InjRV y ★ finished_s ts x y)))%I.
 
-  Global Instance p_inv_timeless γm γr v: TimelessP (p_inv γm γr v).
-  Proof. rewrite /p_inv.  apply uPred.exist_timeless. destruct x as [[[? ?] ?] ?]. apply _. Qed.
-
-  Definition srv_stack_inv (γs γm γr: gname) (s: loc) := (∃ xs, is_stack' (p_inv γm γr) γs xs s)%I.
+  Definition srv_stack_inv γs γm γr s f := (∃ xs, is_stack' (p_inv γm γr f) γs xs s)%I.
 
   Definition srv_tokm_inv γm := (∃ m : tokmR, own γm (● m) ★ [★ map] p ↦ _ ∈ m, ∃ v, p ↦{1/2} v)%I.
 
   Lemma install_push_spec
         (Φ: val → iProp Σ)
         (p: loc) (γs γm γr: gname) (ts: toks)
-        (s: loc) (x: val) :
+        (s: loc) (f x: val) :
     heapN ⊥ N →
-    heap_ctx ★ inv N (srv_stack_inv γs γm γr s ★ srv_tokm_inv γm) ★
-    evm γm p ts ★ installed_s ts x ★
+    heap_ctx ★ inv N (srv_stack_inv γs γm γr s f ★ srv_tokm_inv γm) ★
+    evm γm p ts ★ installed_s ts f x ★
     p ↦{1/2} InjLV x ★ ((∃ hd, evs γs hd #p) -★ Φ #())
     ⊢ WP push #s #p {{ Φ }}.
   Proof.
     iIntros (HN) "(#Hh & #? & Hpm & Hs & Hp & HΦ)".
     rewrite /srv_stack_inv.
-    iDestruct (push_spec N (p_inv γm γr) (fun v => (∃ hd, evs γs hd #p) ★ v = #())%I
+    iDestruct (push_spec N (p_inv γm γr f) (fun v => (∃ hd, evs γs hd #p) ★ v = #())%I
                with "[-HΦ]") as "Hpush"=>//.
     - iFrame "Hh". iSplitL "Hp Hs Hpm"; last eauto.
       iExists ts. iExists p. iSplit=>//. iFrame "Hpm".
@@ -133,35 +137,37 @@ Section proof.
       by iApply "HΦ".
   Qed.
 
-  Definition installed_recp (ts: toks) (x: val) :=
-    let '(γx, _, γ3, _) := ts in (own γ3 (Excl ()) ★ own γx ((1/2)%Qp, DecAgree x))%I.
+  Definition installed_recp (ts: toks) (x: val) (Q: val → val → iProp Σ) :=
+    let '(γx, _, γ3, _, γq) := ts in
+    (own γ3 (Excl ()) ★ own γx ((1/2)%Qp, DecAgree x) ★ saved_prop_own γq (Q x))%I.
 
   Lemma install_spec
-        (Φ: val → iProp Σ)
-        (x: val) (γs γm γr: gname) (s: loc):
+        (Φ: val → iProp Σ) P Q
+        (f x: val) (γs γm γr: gname) (s: loc):
     heapN ⊥ N →
-    heap_ctx ★ inv N (srv_stack_inv γs γm γr s ★ srv_tokm_inv γm) ★ P x ★
-    (∀ (p: loc) (ts: toks), installed_recp ts x -★ evm γm p ts -★(∃ hd, evs γs hd #p) -★ Φ #p)
+    heap_ctx ★ inv N (srv_stack_inv γs γm γr s f ★ srv_tokm_inv γm) ★ P x ★ ({{ R ★ P x }} f x {{ v, R ★ Q x v }}) ★
+    (∀ (p: loc) (ts: toks), installed_recp ts x Q -★ evm γm p ts -★(∃ hd, evs γs hd #p) -★ Φ #p)
     ⊢ WP install x #s {{ Φ }}.
   Proof.
-    iIntros (HN) "(#Hh & #? & Hpx & HΦ)".
+    iIntros (HN) "(#Hh & #? & Hpx & Hf & HΦ)".
     wp_seq. wp_let. wp_alloc p as "Hl".
     iApply pvs_wp.
     iVs (own_alloc (Excl ())) as (γ1) "Ho1"; first done.
     iVs (own_alloc (Excl ())) as (γ3) "Ho3"; first done.
     iVs (own_alloc (Excl ())) as (γ4) "Ho4"; first done.
     iVs (own_alloc (1%Qp, DecAgree x)) as (γx) "Hx"; first done.
-    iInv N as ">[Hrs Hm]" "Hclose".
+    iVs (saved_prop_alloc (F:=(cofe_funCF val idCF)) (Q x)%I) as (γq) "#?".
+    iInv N as "[Hrs >Hm]" "Hclose".
     iDestruct "Hm" as (m) "[Hm HRm]".
     destruct (m !! p) eqn:Heqn.
     - (* old name *)
       iDestruct (big_sepM_delete (fun p _ => ∃ v : val, p ↦{1 / 2} v)%I m with "HRm") as "[Hp HRm]"=>//.
       iDestruct "Hp" as (?) "Hp". iExFalso. iApply bogus_heap; last by iFrame "Hh Hl Hp". auto.
     - (* fresh name *)
-      iDestruct (evmap_alloc _ _ _ m p (γx, γ1, γ3, γ4) with "[Hm]") as "==>[Hm1 Hm2]"=>//.
+      iDestruct (evmap_alloc _ _ _ m p (γx, γ1, γ3, γ4, γq) with "[Hm]") as "==>[Hm1 Hm2]"=>//.
       iDestruct "Hl" as "[Hl1 Hl2]".
       iVs ("Hclose" with "[HRm Hm1 Hl1 Hrs]").
-      + iNext. iFrame. iExists ({[p := (1%Qp, DecAgree (γx, γ1, γ3, γ4))]} ⋅ m). iFrame.
+      + iNext. iFrame. iExists ({[p := (1%Qp, DecAgree (γx, γ1, γ3, γ4, γq))]} ⋅ m). iFrame.
         rewrite <-(insert_singleton_op m)=>//.
         iDestruct (big_sepM_insert _ m with "[-]") as "H"=>//.
         iSplitL "Hl1"; last by iAssumption. eauto.
@@ -171,83 +177,84 @@ Section proof.
         iVsIntro. wp_let. wp_bind ((push _) _).
         iApply install_push_spec=>//.
         iFrame "#". rewrite /evm /installed_s.
-        iFrame "Hev1 Hx1 Hpx Ho1 Ho4 Hl2".
+        iFrame.
+        iSplitL "Hpx Hx1 Hf".
+        { iExists P, Q. by iFrame. }
         iIntros "Hhd". wp_seq. iVsIntro.
-        iSpecialize ("HΦ" $! p (γx, γ1, γ3, γ4) with "[-Hev2 Hhd]")=>//.
-        { rewrite /installed_recp. iFrame. }
-        by iApply ("HΦ" with "Hev2").
+        iSpecialize ("HΦ" $! p (γx, γ1, γ3, γ4, γq) with "[-Hev1 Hhd]")=>//.
+        { rewrite /installed_recp. iFrame. iFrame "#". }
+        by iApply ("HΦ" with "Hev1").
   Qed.
 
   Lemma loop_iter_list_spec Φ (f: val) (s hd: loc) (γs γm γr: gname) xs:
-    heapN ⊥ N → (∀ x:val, {{ R ★ P x }} f x {{ v, R ★ Q x v }}) ★
-    heap_ctx ★ inv N (srv_stack_inv γs γm γr s ★ srv_tokm_inv γm) ★ own γr (Excl ()) ★ R ★
+    heapN ⊥ N →
+    heap_ctx ★ inv N (srv_stack_inv γs γm γr s f ★ srv_tokm_inv γm) ★ own γr (Excl ()) ★ R ★
     is_list' γs hd xs ★ (own γr (Excl ()) -★ R -★ Φ #())
     ⊢ WP doOp f {{ f', WP iter #hd f' {{ Φ }} }}.
   Proof.
-    iIntros (HN) "(#Hf & #? & #? & Ho2 & HR & Hlist' & HΦ)".
+    iIntros (HN) "(#Hf & #? & Ho2 & HR & Hlist' & HΦ)".
     iApply pvs_wp.
     iDestruct (dup_is_list' with "[Hlist']") as "==>[Hl1 Hl2]"; first by iFrame.
     iDestruct (dup_is_list' with "[Hl2]") as "==>[Hl2 Hl3]"; first by iFrame.
     iVsIntro. wp_seq.
-    iDestruct (iter_spec _ (p_inv γm γr) (fun v => v = #() ★ own γr (Excl ()) ★ R)%I γs s
-                         ((∀ x:val, {{ R ★ P x }} f x {{ v, R ★ Q x v }}) ★
-                          is_list' γs hd xs ★ own γr (Excl ()) ★ R)%I (srv_tokm_inv γm) xs hd
+    iDestruct (iter_spec _ (p_inv γm γr f) (fun v => v = #() ★ own γr (Excl ()) ★ R)%I γs s
+                         (is_list' γs hd xs ★ own γr (Excl ()) ★ R)%I (srv_tokm_inv γm) xs hd
                          (doOp' f) (doOp' f)
                          with "[-Hl1 HΦ]") as "Hiter"=>//.
     - rewrite /f_spec.
-      iIntros (Φ' p _ Hin) "(#Hh & #? & (#Hf & Hls & Ho2 & HR) & HΦ')".
-      wp_let. wp_bind (! _)%E. iInv N as ">[Hs Hm]" "Hclose".
-      iDestruct "Hs" as (xs' hd') "[Hhd [Hxs HRs]]".
+      iIntros (Φ' p _ Hin) "(#Hh & #? & (Hls & Ho2 & HR) & HΦ')".
+      wp_let. wp_bind (! _)%E. iInv N as "[Hs >Hm]" "Hclose".
+      iDestruct "Hs" as (xs' hd') "[>Hhd [>Hxs HRs]]".
       iDestruct (dup_is_list' with "[Hls]") as "==>[Hls1 Hls2]"; first by iFrame.
-      iDestruct "HRs" as (m) "[Hom HRs]".
-      iDestruct (access with "[Hom HRs Hls1]") as (hd'' [q x]) "[Hrest [Hhd'' [% Hom]]]"=>//; first by iFrame.
-      iDestruct "Hhd''" as "(% & H & Hphd)". inversion H2. subst.
-      iDestruct "H" as (ts p'') "[% [Hev [Hp | [Hp | [Hp | Hp]]]]]"; subst.
-      + iDestruct "Hp" as (y) "(Hp & Hs)".
+      iDestruct "HRs" as (m) "[>Hom HRs]".
+      (* acccess *)
+      iDestruct (access with "[Hom HRs Hls1]") as (hd'' ?) "(Hrest & HRx & % & Hom)"=>//; first iFrame.
+      iDestruct "HRx" as (v') "[>% [Hpinv' >Hhd'']]". inversion H1. subst.
+      iDestruct "Hpinv'" as (ts p'') "[>% [>Hevm [Hp | [Hp | [Hp | Hp]]]]]"; subst.
+      + iDestruct "Hp" as (y) "(>Hp & Hs)".
         wp_load. iVs ("Hclose" with "[-HΦ' Ho2 HR Hls2]").
         { iNext. iFrame. iExists xs', hd'.
           iFrame "Hhd Hxs". iExists m.
-          iFrame "Hom". iDestruct (big_sepM_delete _ m with "[Hrest Hphd Hev Hp Hs]") as "?"=>//.
+          iFrame "Hom". iDestruct (big_sepM_delete _ m with "[Hrest Hhd'' Hevm Hp Hs]") as "?"=>//.
           iFrame. iExists #p''. iSplitR; first done. iExists ts, p''.
           iSplitR; first done. iFrame. iLeft. iExists y. iFrame. }
         iVsIntro. wp_match. iApply "HΦ'". by iFrame.
       + iDestruct "Hp" as (x') "(Hp & Hs)".
-        wp_load. destruct ts as [[[γx γ1] γ3] γ4].
-        iDestruct "Hs" as "(Hx & Hpx & Ho1 & Ho4)".
-        iDestruct (dup_ev with "Hev") as "==>[Hev1 Hev2]".
+        wp_load. destruct ts as [[[[γx γ1] γ3] γ4] γq].
+        iDestruct "Hs" as  (P Q) "(Hx & Hpx & Hf & HoQ& Ho1 & Ho4)".
+        iDestruct (dup_ev with "Hevm") as "==>[Hevm1 Hevm2]".
         iAssert (|=r=> own γx (((1/2/2)%Qp, DecAgree x') ⋅
                                ((1/2/2)%Qp, DecAgree x')))%I with "[Hx]" as "==>[Hx1 Hx2]".
         { iDestruct (own_update with "Hx") as "?"; last by iAssumption.
           rewrite -{1}(Qp_div_2 (1/2)%Qp).
           by apply pair_l_frac_op'. }
-        iVs ("Hclose" with "[-Hls2 Ho1 Hx2 HR Hev2 Hpx HΦ']").
+        iVs ("Hclose" with "[-Hf Hls2 Ho1 Hx2 HR Hevm2 HoQ Hpx HΦ']").
         { iNext. iFrame. iExists xs', hd'.
           iFrame "Hhd Hxs". iExists m.
           iFrame "Hom". iDestruct (big_sepM_delete _ m with "[-]") as "?"=>//.
           simpl. iFrame. iExists #p''. iSplitR; auto. rewrite /allocated.
-          iExists (γx, γ1, γ3, γ4), p''. iSplitR; auto.
+          iExists (γx, γ1, γ3, γ4, γq), p''. iSplitR; auto.
           iFrame. iRight. iRight. iLeft. iExists x'. iFrame. }
         iVsIntro. wp_match.
-        wp_bind (f _). iApply wp_wand_r. iSplitL "Hpx HR".
+        wp_bind (f _). iApply wp_wand_r. iSplitL "Hpx Hf HR".
         { iApply "Hf". iFrame. }
         iIntros (v) "[HR HQ]".
-        wp_value. iVsIntro. iInv N as ">[Hs Hm]" "Hclose".
-        iDestruct "Hs" as (xs'' hd''') "[Hhd [Hxs HRs]]".
-        iDestruct "HRs" as (m') "[Hom HRs]".
+        wp_value. iVsIntro. iInv N as "[Hs >Hm]" "Hclose".
+        iDestruct "Hs" as (xs'' hd''') "[>Hhd [>Hxs HRs]]".
+        iDestruct "HRs" as (m') "[>Hom HRs]".
         iDestruct (dup_is_list' with "[Hls2]") as "==>[Hls2 Hls3]"; first by iFrame.
-        iDestruct (access with "[Hom HRs Hls2]") as (hd'''' [? ?]) "[Hrest [Hhd'' [% Hom]]]"=>//;
-         first by iFrame.
-        iDestruct "Hhd''" as "(% & H & Hphd)". inversion H4. subst.
-        iDestruct "H" as ([[[γx' γ1'] γ3'] γ4'] p'''') "[% [Hev Hps]]".
-        inversion H5. subst.
-        destruct (decide (γ1 = γ1' ∧ γx = γx' ∧ γ3 = γ3' ∧ γ4 = γ4')) as [[? [? [? ?]]]|Hneq]; subst.
+        iDestruct (access with "[Hom HRs Hls2]") as (hd'''' q) "(Hrest & HRx & % & Hom)"=>//; first iFrame.
+        iDestruct "HRx" as (v'') "[>% [Hpinv' >Hhd'']]". inversion H2. subst.
+        iDestruct "Hpinv'" as ([[[[γx' γ1'] γ3'] γ4'] γq'] p'''') "[>% [>Hevm Hps]]".
+        inversion H3. subst.
+        destruct (decide (γ1 = γ1' ∧ γx = γx' ∧ γ3 = γ3' ∧ γ4 = γ4' ∧ γq = γq')) as [[? [? [? [? ?]]]]|Hneq]; subst.
         {
           iDestruct "Hps" as "[Hp | [Hp | [Hp | Hp]]]".
-          * iDestruct "Hp" as (?) "(_ & Ho1' & _)".
+          * iDestruct "Hp" as (?) "(_ & >Ho1' & _)".
             iApply excl_falso. iFrame.
-          * iDestruct "Hp" as (?) "(_ & _ & _ & Ho1' & _)".
+          * iDestruct "Hp" as (?) "[>? Hs]". iDestruct "Hs" as (? ?) "(_ & _ & _ & _ & >Ho1' & _)".
             iApply excl_falso. iFrame.
-          * iDestruct "Hp" as (x5) "(Hp & Hx & Ho2 & Ho4)".
+          * iDestruct "Hp" as (x5) ">(Hp & Hx & Ho2 & Ho4)".
             iDestruct "Hm" as (m2) "[Hom2 HRm]".
             destruct (m2 !! p'''') eqn:Heqn.
             {
@@ -266,55 +273,59 @@ Section proof.
                 iExists m'. iFrame.
                 iDestruct (big_sepM_delete _ m' with "[-]") as "?"=>//.
                 { simpl. iFrame. iExists #p''''.
-                  iSplitR; first auto. iExists (γx', γ1', γ3', γ4'), p''''.
-                  iSplitR; first auto. iFrame "Hev". iRight. iRight.
+                  iSplitR; first auto. iExists (γx', γ1', γ3', γ4', γq'), p''''.
+                  iSplitR; first auto. iFrame "Hevm". iRight. iRight.
                   iRight. iExists x5, v. iFrame.
+                  iExists Q. iFrame.                  
                 }
               }
               iApply "HΦ'". by iFrame.
             }
             { iExFalso. iApply (map_agree_none' _ _ _ m2)=>//. iFrame. }
-          * iDestruct "Hp" as (? ?) "(_ & _ & _ & Ho1' & _)".
+          * iDestruct "Hp" as (? ?) "[? Hs]". iDestruct "Hs" as (?) "(_ & _ & _ & >Ho1' & _)".
             iApply excl_falso. iFrame.
         }
-        { iDestruct (ev_agree with "[Hev2 Hev]") as "==>[_ [_ %]]"; first iFrame.
-          inversion H6. subst. by contradiction Hneq. }
-      + destruct ts as [[[γx γ1] γ3] γ4]. iDestruct "Hp" as (y) "(_ & _ & Ho2' & _)".
+        { iDestruct (ev_agree with "[Hevm Hevm2]") as "==>[_ [_ %]]"; first iFrame.
+          inversion H4. subst. by contradiction Hneq. }
+      + destruct ts as [[[[γx γ1] γ3] γ4] γq]. iDestruct "Hp" as (y) "(_ & _ & >Ho2' & _)".
         iApply excl_falso. iFrame.
-      + destruct ts as [[[γx γ1] γ3] γ4]. iDestruct "Hp" as (x' y) "(Hp & Hx & HQxy & Ho1 & Ho4)".
+      + destruct ts as [[[[γx γ1] γ3] γ4] γq]. iDestruct "Hp" as (x' y) "[Hp Hs]".
+        iDestruct "Hs" as (Q) "(>Hx & HoQ & HQxy & >Ho1 & >Ho4)".
         wp_load. iVs ("Hclose" with "[-HΦ' HR Ho2 Hls2]").
         { iNext. iFrame. iExists xs', hd'.
           iFrame "Hhd Hxs". iExists m.
           iFrame "Hom". iDestruct (big_sepM_delete _ m with "[-]") as "?"=>//.
-          iFrame. iExists #p''. iSplitR; first auto. iExists (γx, γ1, γ3, γ4), p''.
-          iSplitR; auto. iFrame. iRight. iRight. iRight. iExists x', y. iFrame. }
+          iFrame. iExists #p''. iSplitR; first auto. iExists (γx, γ1, γ3, γ4, γq), p''.
+          iSplitR; auto. iFrame. iRight. iRight. iRight. iExists x', y. iFrame.
+          iExists Q. iFrame. }
         iVsIntro. wp_match. iApply "HΦ'". by iFrame.
     - apply to_of_val.
-    - rewrite /srv_stack_inv. iFrame "#". iFrame. iIntros "[_ (? & ? & ?)]". by iFrame.
+    - rewrite /srv_stack_inv. iFrame "#". iFrame. iIntros "(? & ? & ?)". by iFrame.
     - iApply wp_wand_r. iSplitL "Hiter"; first done.
       iIntros (?) "[% [Ho2 HR]]". subst. iApply ("HΦ" with "Ho2 HR").
   Qed.
 
-  Definition own_γ3 (ts: toks) := let '(_, _, γ3, _) := ts in own γ3 (Excl ()).
+  Definition own_γ3 (ts: toks) := let '(_, _, γ3, _, _) := ts in own γ3 (Excl ()).
   Definition finished_recp (ts: toks) (x y: val) :=
-    let '(γx, _, _, _) := ts in (own γx ((1 / 2)%Qp, DecAgree x) ★ Q x y)%I.
+    let '(γx, _, _, _, γq) := ts in
+    (∃ Q, own γx ((1 / 2)%Qp, DecAgree x) ★ saved_prop_own γq (Q x) ★ Q x y)%I.
 
   Lemma try_srv_spec Φ (s: loc) (lk: val) (f: val)
         (γs γr γm γlk: gname):
-    heapN ⊥ N → (∀ x:val, {{ R ★ P x }} f x {{ v, R ★ Q x v }}) ★
-    heap_ctx ★ inv N (srv_stack_inv γs γm γr s ★ srv_tokm_inv γm) ★
+    heapN ⊥ N →
+    heap_ctx ★ inv N (srv_stack_inv γs γm γr s f ★ srv_tokm_inv γm) ★
     is_lock N γlk lk (own γr (Excl ()) ★ R) ★ Φ #()
     ⊢ WP try_srv lk #s f {{ Φ }}.
   Proof.
-    iIntros (?) "(#? & #? & #? & #? & HΦ)".
+    iIntros (?) "(#? & #? & #? & HΦ)".
     wp_seq. wp_let. wp_let.
     wp_bind (try_acquire _). iApply try_acquire_spec.
     iFrame "#". iSplit; last by wp_if.
     (* acquired the lock *)
     iIntros "Hlocked [Ho2 HR]".
     wp_if. wp_bind (! _)%E.
-    iInv N as ">[H Hm]" "Hclose".
-    iDestruct "H" as (xs' hd') "[Hs [Hxs HRs]]".
+    iInv N as "[H >Hm]" "Hclose".
+    iDestruct "H" as (xs' hd') "[>Hs [>Hxs HRs]]".
     wp_load. iDestruct (dup_is_list' with "[Hxs]") as "==>[Hxs1 Hxs2]"; first by iFrame.
     iVs ("Hclose" with "[Hs Hxs1 HRs Hm]").
     { iNext. iFrame. iExists xs', hd'. by iFrame. }
@@ -332,39 +343,38 @@ Section proof.
     
   Lemma loop_spec Φ (p s: loc) (lk: val) (f: val)
         (γs γr γm γlk: gname) (ts: toks):
-    heapN ⊥ N → (∀ x:val, {{ R ★ P x }} f x {{ v, R ★ Q x v }}) ★
-    heap_ctx ★ inv N (srv_stack_inv γs γm γr s ★ srv_tokm_inv γm) ★
+    heapN ⊥ N →
+    heap_ctx ★ inv N (srv_stack_inv γs γm γr s f ★ srv_tokm_inv γm) ★
     is_lock N γlk lk (own γr (Excl ()) ★ R) ★
     own_γ3 ts ★ evm γm p ts ★
     (∃ hd, evs γs hd #p) ★ (∀ x y, finished_recp ts x y -★ Φ y)
     ⊢ WP loop f #p #s lk {{ Φ }}.
   Proof.
-    iIntros (HN) "(#Hf & #Hh & #? & #? & Ho3 & Hev & Hhd & HΦ)".
+    iIntros (HN) "(#Hh & #? & #? & Ho3 & Hev & Hhd & HΦ)".
     iLöb as "IH". wp_rec. repeat wp_let.
-    wp_bind (! _)%E. iInv N as ">[Hinv ?]" "Hclose".
-    iDestruct "Hinv" as (xs hd) "[Hs [Hxs HRs]]".
-    iDestruct "HRs" as (m) "[Hom HRs]".
+    wp_bind (! _)%E. iInv N as "[Hinv >?]" "Hclose".
+    iDestruct "Hinv" as (xs hd) "[>Hs [>Hxs HRs]]".
+    iDestruct "HRs" as (m) "[>Hom HRs]".
     iDestruct "Hhd" as (hdp ?) "Hhd".
     destruct (m !! hdp) eqn:Heqn.
-    - iDestruct (big_sepM_delete _ m with "HRs") as "[Hp Hrs]"=>//.
-      iDestruct "Hp" as (?) "[% [Hpr ?]]"; subst.
-      iDestruct "Hpr" as (ts' p') "(% & Hp' & Hp)".
+    - iDestruct (big_sepM_delete_later _ m with "HRs") as "[Hp Hrs]"=>//.
+      iDestruct "Hp" as (?) "[>% [Hpr ?]]"; subst.
+      iDestruct "Hpr" as (ts' p') "(>% & >Hp' & Hp)".
       subst. iDestruct (map_agree_eq' _ _ γs m with "[Hom Hhd]") as "(Hom & Hhd & %)"=>//.
       { iFrame. rewrite /ev. eauto. }
-      inversion H2. subst.
+      inversion H0. subst.
       iDestruct (ev_agree with "[Hev Hp']") as "==>[Hγs2 [Hγs %]]"; first iFrame. subst.
-      destruct ts as [[[γx γ1] γ3] γ4].
+      destruct ts as [[[[γx γ1] γ3] γ4] γq].
       iDestruct "Hp" as "[Hp | [Hp | [ Hp | Hp]]]".
-      + iDestruct "Hp" as (?) "(_ & _ & Ho3')".
+      + iDestruct "Hp" as (?) "(_ & _ & >Ho3')".
         iApply excl_falso. iFrame.
-      + iDestruct "Hp" as (x) "(Hp & Hx & Ho1 & Ho4)".
+      + iDestruct "Hp" as (x) "(>Hp & Hs')".
         wp_load. iVs ("Hclose" with "[-Hγs2 Ho3 HΦ Hhd]").
         { iNext. iFrame. iExists xs, hd. iFrame. iExists m. iFrame.
           iDestruct (big_sepM_delete _ m with "[-]") as "?"=>//.
-          iFrame. iExists #p'. iSplitR; first auto. iExists (γx, γ1, γ3, γ4), p'.
+          iFrame. iExists #p'. iSplitR; first auto. iExists (γx, γ1, γ3, γ4, γq), p'.
           iSplitR; first auto. iFrame.
-          iRight. iLeft. iExists x.
-          iFrame. }
+          iRight. iLeft. iExists x. iFrame. }
         iVsIntro. wp_match.
         wp_bind (try_srv _ _ _). iApply try_srv_spec=>//.
         iFrame "#". wp_seq.
@@ -375,36 +385,35 @@ Section proof.
         iVs ("Hclose" with "[-Hγs Ho3 HΦ Hhd]").
         { iNext. iFrame. iExists xs, hd. iFrame. iExists m. iFrame.
           iDestruct (big_sepM_delete _ m with "[-]") as "?"=>//.
-          iFrame. iExists #p'. iSplitR; auto. iExists (γx, γ1, γ3, γ4), p'.
+          iFrame. iExists #p'. iSplitR; auto. iExists (γx, γ1, γ3, γ4, γq), p'.
           iSplitR; first auto. iFrame.
-          iRight. iRight. iLeft. iExists x. iFrame.
-        }
+          iRight. iRight. iLeft. iExists x. iFrame. }
         iVsIntro. wp_match.
         wp_bind (try_srv _ _ _). iApply try_srv_spec=>//.
         iFrame "#". wp_seq.
         iAssert (∃ hd, evs γs hd #p')%I with "[Hhd]" as "Hhd"; eauto.
         by iApply ("IH" with "Ho3 Hγs Hhd").
-      + iDestruct "Hp" as (x y) "(Hp & Hx & HQ & Ho1 & Ho4)".
-          wp_load.
-          iVs ("Hclose" with "[-Hγs Ho4 HΦ Hx HQ]").
+       + iDestruct "Hp" as (x y) "[>Hp Hs']". iDestruct "Hs'" as (Q) "(>Hx & HoQ & HQ & >Ho1 & >Ho4)".
+          wp_load. iVs ("Hclose" with "[-Hγs Ho4 HΦ Hx HoQ HQ]").
           { iNext. iFrame. iExists xs, hd. iFrame. iExists m. iFrame.
             iDestruct (big_sepM_delete _ m with "[-]") as "?"=>//.
-            iFrame. iExists #p'. iSplitR; auto. iExists (γx, γ1, γ3, γ4), p'.
+            iFrame. iExists #p'. iSplitR; auto. iExists (γx, γ1, γ3, γ4, γq), p'.
             iSplitR; first auto. iFrame.
             iLeft. iExists y. iFrame. }
           iVsIntro. wp_match. iApply ("HΦ" with "[-]"). iFrame.
+          iExists Q. iFrame.
     - iExFalso. iApply (map_agree_none' _ _ _ m)=>//. iFrame "Hom".
       rewrite /ev. eauto.
   Qed.
 
-  Definition is_flatter (fl: val) :=
-    (∀ f:val , WP fl f {{ f', □ ((∀ x:val, {{ R ★ P x }} f x {{ v, R ★ Q x v }}) →
-                                 (∀ x:val, {{ P x }} f' x {{ v, Q x v }}))}})%I.
+  Definition flatten (f' f: val) :=
+    (∀ P Q, (∀ x:val, {{ R ★ P x }} f x {{ v, R ★ Q x v }}) →
+            (∀ x:val, {{ P x }} f' x {{ v, ▷ Q x v }}))%I.
 
-  Lemma mk_flat_spec:
+  Lemma mk_flat_spec (f: val) :
     ∀ (Φ: val → iProp Σ),
       heapN ⊥ N →
-      heap_ctx ★ R ★ (∀ fl, is_flatter fl -★ Φ fl) ⊢ WP mk_flat #() {{ Φ }}.
+      heap_ctx ★ R ★ (∀ f', □ flatten f' f -★ Φ f') ⊢ WP mk_flat f {{ Φ }}.
   Proof.
     iIntros (Φ HN) "(#Hh & HR & HΦ)".
     iVs (own_alloc (Excl ())) as (γr) "Ho2"; first done.
@@ -415,22 +424,25 @@ Section proof.
     iApply (newlock_spec _ (own γr (Excl ()) ★ R))%I=>//.
     iFrame "Hh Ho2 HR". iIntros (lk γlk) "#Hlk".
     wp_let. wp_bind (new_stack _).
-    iApply (new_stack_spec' _ (p_inv γm γr))=>//.
+    iApply (new_stack_spec' _ (p_inv γm γr f))=>//.
     iFrame "Hh Hm". iIntros (γ s) "#Hss".
-    wp_let. iVsIntro. iApply "HΦ". rewrite /is_flatter. iIntros (f). wp_let.
-    iVsIntro. iAlways. iIntros "#Hf".
+    wp_let. iVsIntro. iApply "HΦ". rewrite /flatten.
+    iAlways. iIntros (P Q) "#Hf".
     iIntros (x) "!# Hp". wp_let.
     wp_bind ((install _) _).
-    iApply install_spec=>//.
-    iFrame "#". iFrame "Hp". iIntros (p [[[γx γ1] γ3] γ4]) "[Ho3 Hx] Hev Hhd".
+    iApply (install_spec _ P Q)=>//.
+    iFrame "#". iFrame "Hp". iSplitR; first iApply "Hf".
+    iIntros (p [[[[γx γ1] γ3] γ4] γq]) "(Ho3 & Hx & HoQ) Hev Hhd".
     wp_let. iApply loop_spec=>//.
     iFrame "#". iFrame.
-    iIntros (? ?) "[Hx' HQ]".
-    destruct (decide (x = a)) as [->|Hneq]; first done.
-    { iExFalso. iCombine "Hx" "Hx'" as "Hx".
+    iIntros (? ?) "Hs".
+    iDestruct "Hs" as (Q') "(Hx' & HoQ' & HQ')".
+    destruct (decide (x = a)) as [->|Hneq].
+    - iDestruct (saved_prop_agree with "[HoQ HoQ']") as "Heq"; first by iFrame.
+      iNext. admit. (* iRewrite "Heq" in "HQ'". *)
+    - iExFalso. iCombine "Hx" "Hx'" as "Hx".
       iDestruct (own_valid with "Hx") as %[_ H1].
       rewrite pair_op //= dec_agree_ne in H1=>//.
-    }
-  Qed.
+  Admitted.
 
 End proof.
